Make clos_number leave gaps for clos_to_bvl's daisy chaining

compiler/backend/proofs/clos_numberProofScript.sml
@@ -160,11 +160,20 @@ val (v_rel_rules,v_rel_ind,v_rel_cases) = Hol_reln `
    ⇒
    v_rel max_app (Recclosure p argenv env es k) (Recclosure p' argenv' env' es' k))`
 
+val compile_inc_def = Define `
+  compile_inc n xs =
+    (* leave space in the naming for the daisy chaining of clos_to_bvl *)
+    let n1 = 2 * MAX (LENGTH xs) 1 + n in
+    let (m,ys) = renumber_code_locs_list n1 xs in
+      (* embed the name of the first free slot (n) in the code *)
+      (* no code will be generated for this pure Const expression *)
+      (m, Op None (Const (&n)) [] :: ys)`;
+
 val state_rel_def = Define `
   state_rel (s:(num#'c,'ffi) closSem$state) (t:('c,'ffi) closSem$state) <=>
     (s.clock = t.clock) /\ (s.ffi = t.ffi) /\ (t.max_app = s.max_app) /\
-    s.compile = state_cc (ignore_table renumber_code_locs_list) t.compile /\
-    t.compile_oracle = state_co (ignore_table renumber_code_locs_list) s.compile_oracle /\
+    s.compile = state_cc (ignore_table compile_inc) t.compile /\
+    t.compile_oracle = state_co (ignore_table compile_inc) s.compile_oracle /\
     fmap_rel (ref_rel (v_rel s.max_app)) s.refs t.refs ∧
     EVERY2 (OPTREL (v_rel s.max_app)) s.globals t.globals /\
     (∀n. SND (SND (s.compile_oracle n )) = [] ∧
@@ -480,7 +489,7 @@ val do_install = Q.prove(
    (∀e1 t1. do_install x1 s1 = (Rval e1,t1) ⇒
      ∃e2 t2. do_install x2 s2 = (Rval e2,t2) ∧
              ¬contains_App_SOME t1.max_app (e1) ∧ t1.max_app = s1.max_app ∧
-             e2 = SND (renumber_code_locs_list (FST(FST(s1.compile_oracle 0))) e1) ∧
+             e2 = SND (compile_inc (FST(FST(s1.compile_oracle 0))) e1) ∧
              state_rel t1 t2)`,
   strip_tac
   \\ `∃res. do_install x1 s1 = res` by fs[]
@@ -492,8 +501,8 @@ val do_install = Q.prove(
   \\ imp_res_tac state_rel_max_app \\ fs[]
   \\ imp_res_tac state_rel_clock \\ fs[]
   \\ fs[shift_seq_def]
-  \\ `s2.compile_oracle = state_co (ignore_table renumber_code_locs_list) s1.compile_oracle` by fs[state_rel_def]
-  \\ `s1.compile = state_cc (ignore_table renumber_code_locs_list) s2.compile` by fs[state_rel_def]
+  \\ `s2.compile_oracle = state_co (ignore_table compile_inc) s1.compile_oracle` by fs[state_rel_def]
+  \\ `s1.compile = state_cc (ignore_table compile_inc) s2.compile` by fs[state_rel_def]
   \\ fs[]
   \\ qpat_x_assum`state_co _ _ _ = _`mp_tac
   \\ simp[Once state_co_def]
@@ -512,7 +521,9 @@ val do_install = Q.prove(
   \\ fs[CaseEq"bool"]
   \\ fs[ignore_table_def]
   \\ pairarg_tac \\ fs[] \\ rveq
-  \\ imp_res_tac renumber_code_locs_list_length
+  \\ rename [`_ = (st1,code1)`]
+  \\ `code1 <> []` by
+    (fs [compile_inc_def] \\ pairarg_tac \\ fs [] \\ rveq \\ fs [])
   \\ fs[state_rel_def,state_co_def,ignore_table_def]
   \\ metis_tac[FUPDATE_LIST_THM,FST,SND,DECIDE``(n+1n)+1 = n+2``,LENGTH_NIL] );
 
@@ -670,26 +681,47 @@ val renumber_code_locs_correct = Q.store_thm("renumber_code_locs_correct",
       \\ drule (GEN_ALL do_install) \\ fs[]
       \\ imp_res_tac EVERY2_REVERSE \\ pop_assum kall_tac
       \\ disch_then drule
-      \\ strip_tac
-      \\ fsrw_tac[DNF_ss][case_eq_thms,pair_case_eq] \\ rfs[] \\ fs[]
+      \\ reverse (strip_tac
+        \\ fsrw_tac[DNF_ss][case_eq_thms,pair_case_eq]
+        \\ rfs[] \\ fs[] \\ rveq \\ fs[])
+      THEN1
+       (Cases_on `err` \\ fs []
+        \\ imp_res_tac do_install_not_Rraise \\ fs []
+        \\ rename1 `aa = Rtimeout_error ==> _`
+        \\ Cases_on `aa` \\ fs []
+        \\ imp_res_tac do_install_not_Rffi_error \\ fs[])
+      \\ first_x_assum drule
+      \\ fs [compile_inc_def]
+      \\ qmatch_goalsub_abbrev_tac`renumber_code_locs_list nn`
+      \\ disch_then(qspec_then`nn`strip_assume_tac)
       \\ rveq \\ fs[]
-      \\ TRY (
-         first_x_assum drule
-         \\ qmatch_goalsub_abbrev_tac`renumber_code_locs_list nn`
-         \\ disch_then(qspec_then`nn`strip_assume_tac)
-         \\ rveq \\ fs[]
-         THEN (
-           Q.ISPEC_THEN`v''`FULL_STRUCT_CASES_TAC SNOC_CASES
-           >- (
-             imp_res_tac evaluate_IMP_LENGTH
-             \\ fs[do_install_def,CaseEq"list",CaseEq"option",CaseEq"prod"]
-             \\ pairarg_tac \\ fs[CaseEq"bool",CaseEq"option",CaseEq"prod"] )
-           \\ fs[LIST_REL_SNOC] ))
-      \\ Cases_on `err` \\ fs []
-      \\ imp_res_tac do_install_not_Rraise \\ fs []
-      \\ rename1 `aa = Rtimeout_error ==> _`
-      \\ Cases_on `aa` \\ fs []
-      \\ imp_res_tac do_install_not_Rffi_error \\ fs[]) >>
+      THEN1
+       (rename [`LIST_REL (v_rel t1.max_app) a vss`]
+        \\ Q.ISPEC_THEN`vss`FULL_STRUCT_CASES_TAC SNOC_CASES
+        >- (
+          imp_res_tac evaluate_IMP_LENGTH
+          \\ fs[do_install_def,CaseEq"list",CaseEq"option",CaseEq"prod"]
+          \\ pairarg_tac \\ fs[CaseEq"bool",CaseEq"option",CaseEq"prod"] )
+        \\ fs[LIST_REL_SNOC]
+        \\ pairarg_tac \\ fs []
+        \\ once_rewrite_tac [evaluate_CONS]
+        \\ fs [EVAL ``evaluate ([Op None (Const n) []],[],t)``])
+      \\ Q.ISPEC_THEN`v'`FULL_STRUCT_CASES_TAC SNOC_CASES
+      >- (
+        imp_res_tac evaluate_IMP_LENGTH
+        \\ fs[do_install_def,CaseEq"list",CaseEq"option",CaseEq"prod"]
+        \\ pairarg_tac \\ fs[CaseEq"bool",CaseEq"option",CaseEq"prod"] )
+      \\ fs[LIST_REL_SNOC]
+      \\ pairarg_tac \\ fs []
+      \\ once_rewrite_tac [evaluate_CONS]
+      \\ fs [EVAL ``evaluate ([Op None (Const n) []],[],t)``]
+      \\ rename [`LIST_REL _ a vss`]
+      \\ reverse (Q.ISPEC_THEN`vss`FULL_STRUCT_CASES_TAC SNOC_CASES)
+      THEN1 (rewrite_tac [GSYM SNOC,LAST_SNOC] \\ fs [LIST_REL_SNOC])
+      \\ rveq \\ fs [] \\ rveq \\ fs []
+      \\ fs [do_install_def,case_eq_thms]
+      \\ rpt (pairarg_tac \\ fs [])
+      \\ fs [do_install_def,case_eq_thms,bool_case_eq,pair_case_eq]) >>
     srw_tac[][] >>
     first_x_assum(fn th => first_assum(mp_tac o MATCH_MP (ONCE_REWRITE_RULE[GSYM AND_IMP_INTRO]th))) >>
     disch_then(fn th => first_assum(qspec_then`n`STRIP_ASSUME_TAC o MATCH_MP th)) >> rev_full_simp_tac(srw_ss())[] >>
@@ -948,16 +980,16 @@ val renumber_code_locs_esgc_free = Q.store_thm(
 
 val semantics_number = Q.store_thm ("semantics_number",
   `semantics (ffi:'ffi ffi_state) max_app FEMPTY co
-     (state_cc (ignore_table renumber_code_locs_list) cc) xs <> Fail ==>
+     (state_cc (ignore_table compile_inc) cc) xs <> Fail ==>
    ¬contains_App_SOME max_app xs /\
    (∀n.
       SND (SND (co n)) = [] ∧
       ¬contains_App_SOME max_app (FST (SND (co n)))) ==>
    semantics (ffi:'ffi ffi_state) max_app FEMPTY
-     (state_co (ignore_table renumber_code_locs_list) co) cc
+     (state_co (ignore_table compile_inc) co) cc
         (SND (renumber_code_locs_list n xs)) =
    semantics (ffi:'ffi ffi_state) max_app FEMPTY
-     co (state_cc (ignore_table renumber_code_locs_list) cc) xs`
+     co (state_cc (ignore_table compile_inc) cc) xs`
   ,
   strip_tac
   \\ ho_match_mp_tac IMP_semantics_eq
@@ -966,7 +998,7 @@ val semantics_number = Q.store_thm ("semantics_number",
        |> CONJUNCT1 |> SIMP_RULE std_ss [])
   \\ simp []
   \\ qabbrev_tac `ff = initial_state ffi max_app FEMPTY
-       (state_co (ignore_table renumber_code_locs_list) co) cc`
+       (state_co (ignore_table compile_inc) co) cc`
   \\ disch_then (qspec_then `ff k` mp_tac)
   \\ qunabbrev_tac `ff`
   \\ disch_then (qspec_then `n` mp_tac)
